Complete weakening lemma

theories/WLemmata.v
@@ -6,6 +6,8 @@ Require Import util WAst WLiftSubst WTyping.
 
 Section Lemmata.
 
+Open Scope w_scope.
+
 Context `{Sort_notion : Sorts.notion}.
 
 Lemma typing_wf :
@@ -21,6 +23,47 @@ Fixpoint lift_context n Γ : wcontext :=
   | nil => nil
   | A :: Γ => (lift n #|Γ| A) :: (lift_context n Γ)
   end.
+
+Lemma lift_context_length :
+  forall Γ n, #|lift_context n Γ| = #|Γ|.
+Proof.
+  intro Γ. induction Γ ; intro m.
+  - reflexivity.
+  - cbn. f_equal. eapply IHΓ.
+Defined.
+
+Fact safe_nth_lift_context :
+  forall {Γ Δ : wcontext} {n isdecl isdecl'},
+    safe_nth (lift_context #|Γ| Δ) (exist _ n isdecl) =
+    lift #|Γ| (#|Δ| - n - 1) (safe_nth Δ (exist _ n isdecl')).
+Proof.
+  intros Γ Δ. induction Δ.
+  - cbn. intros. bang.
+  - intro n. destruct n ; intros isdecl isdecl'.
+    + cbn. replace (#|Δ| - 0) with #|Δ| by myomega. reflexivity.
+    + cbn. erewrite IHΔ. reflexivity.
+Defined.
+
+Fact lift_context_ex :
+  forall {Δ Ξ : wcontext} {n isdecl isdecl'},
+    lift0 (S n) (safe_nth (lift_context #|Δ| Ξ) (exist _ n isdecl)) =
+    lift #|Δ| #|Ξ| (lift0 (S n) (safe_nth Ξ (exist _ n isdecl'))).
+Proof.
+  intros Δ Ξ n isdecl isdecl'.
+  erewrite safe_nth_lift_context.
+  rewrite <- liftP2 by myomega.
+  cbn.
+  replace (S (n + (#|Ξ| - n - 1)))%nat with #|Ξ|.
+  - reflexivity.
+  - revert n isdecl isdecl'. induction Ξ ; intros n isdecl isdecl'.
+    + cbn. exfalso. abstract easy.
+    + cbn. f_equal.
+      destruct n.
+      * cbn. myomega.
+      * cbn. apply IHΞ.
+        -- cbn in *. myomega.
+        -- cbn in *. myomega.
+Defined.
 
 Definition wapp_context (Γ Γ' : wcontext) : wcontext := (Γ' ++ Γ)%list.
 Notation " Γ  ,,, Γ' " :=
@@ -45,6 +88,249 @@ Lemma meta_ctx_conv :
 Proof.
   intros Σ Γ Δ t A H e.
   destruct e. assumption.
+Defined.
+
+Fact cat_nil :
+  forall {Γ}, Γ ,,, [] = Γ.
+Proof.
+  reflexivity.
+Defined.
+
+Fact nil_cat :
+  forall {Γ}, [] ,,, Γ = Γ.
+Proof.
+  induction Γ.
+  - reflexivity.
+  - cbn. f_equal. assumption.
+Defined.
+
+Fact length_cat :
+  forall {A} {Γ Δ : list A}, #|Γ ++ Δ| = (#|Γ| + #|Δ|)%nat.
+Proof.
+  intros A Γ. induction Γ ; intro Δ.
+  - cbn. reflexivity.
+  - cbn. f_equal. apply IHΓ.
+Defined.
+
+Fact safe_nth_S :
+  forall {A n} {a : A} {l isdecl},
+    ∑ isdecl',
+      safe_nth (a :: l) (exist _ (S n) isdecl) =
+      safe_nth l (exist _ n isdecl').
+Proof.
+  intros A n. induction n ; intros a l isdecl.
+  - cbn. eexists. reflexivity.
+  - eexists. cbn. reflexivity.
+Defined.
+
+Lemma eq_safe_nth' :
+  forall {Γ : wcontext} {n a isdecl isdecl'},
+    safe_nth (a :: Γ) (exist _ (S n) isdecl') =
+    safe_nth Γ (exist _ n isdecl).
+Proof.
+  intros Γ. induction Γ ; intros n A isdecl isdecl'.
+  - exfalso. abstract easy.
+  - destruct n.
+    + reflexivity.
+    + destruct (@safe_nth_S _ (S n) A (a :: Γ) isdecl')
+        as [isecl0 eq].
+      rewrite eq.
+      destruct (@safe_nth_S _ n a Γ isdecl)
+        as [isecl1 eq1].
+      rewrite eq1.
+      apply IHΓ.
+Defined.
+
+Lemma eq_safe_nth :
+  forall {Γ : wcontext} {n A isdecl isdecl'},
+    safe_nth (Γ ,, A) (exist _ (S n) isdecl') =
+    safe_nth Γ (exist _ n isdecl).
+Proof.
+  intros Γ n A isdecl isdecl'.
+  apply eq_safe_nth'.
+Defined.
+
+Fact safe_nth_irr :
+  forall {A n} {l : list A} {isdecl isdecl'},
+    safe_nth l (exist _ n isdecl) =
+    safe_nth l (exist _ n isdecl').
+Proof.
+  intros A n. induction n ; intro l ; destruct l ; intros isdecl isdecl'.
+  all: cbn. all: try bang.
+  - reflexivity.
+  - eapply IHn.
+Defined.
+
+Fact safe_nth_cong_irr :
+  forall {A n m} {l : list A} {isdecl isdecl'},
+    n = m ->
+    safe_nth l (exist _ n isdecl) =
+    safe_nth l (exist _ m isdecl').
+Proof.
+  intros A n m l isdecl isdecl' e.
+  revert isdecl isdecl'.
+  rewrite e. intros isdecl isdecl'.
+  apply safe_nth_irr.
+Defined.
+
+Fact safe_nth_ge :
+  forall {Γ Δ n} { isdecl : n < #|Γ ,,, Δ| } { isdecl' : n - #|Δ| < #|Γ| },
+    n >= #|Δ| ->
+    safe_nth (Γ ,,, Δ) (exist _ n isdecl) =
+    safe_nth Γ (exist _ (n - #|Δ|) isdecl').
+Proof.
+  intros Γ Δ.
+  induction Δ ; intros n isdecl isdecl' h.
+  - cbn in *. revert isdecl'.
+    replace (n - 0) with n by myomega.
+    intros isdecl'. apply safe_nth_irr.
+  - destruct n.
+    + cbn in *. inversion h.
+    + cbn. apply IHΔ. cbn in *. myomega.
+Defined.
+
+Definition ge_sub {Γ Δ n} (isdecl : n < #|Γ ,,, Δ|) :
+  n >= #|Δ| ->  n - #|Δ| < #|Γ|.
+Proof.
+  intro h.
+  rewrite length_cat in isdecl. myomega.
+Defined.
+
+Fact safe_nth_ge' :
+  forall {Γ Δ n} { isdecl : n < #|Γ ,,, Δ| } (h : n >= #|Δ|),
+    safe_nth (Γ ,,, Δ) (exist _ n isdecl) =
+    safe_nth Γ (exist _ (n - #|Δ|) (ge_sub isdecl h)).
+Proof.
+  intros Γ Δ n isdecl h.
+  eapply safe_nth_ge. assumption.
+Defined.
+
+Fact safe_nth_lt :
+  forall {n Γ Δ} { isdecl : n < #|Γ ,,, Δ| } { isdecl' : n < #|Δ| },
+    safe_nth (Γ ,,, Δ) (exist _ n isdecl) =
+    safe_nth Δ (exist _ n isdecl').
+Proof.
+  intros n. induction n ; intros Γ Δ isdecl isdecl'.
+  - destruct Δ.
+    + cbn in *. inversion isdecl'.
+    + cbn. reflexivity.
+  - destruct Δ.
+    + cbn in *. inversion isdecl'.
+    + cbn. eapply IHn.
+Defined.
+
+Fact ident_neq_fresh :
+  forall {Σ id ty d},
+    lookup_glob Σ id = Some ty ->
+    fresh_glob (dname d) Σ ->
+    ident_eq id (dname d) = false.
+Proof.
+  intro Σ. induction Σ ; intros id ty d h hf.
+  - cbn in h. discriminate h.
+  - cbn in h. dependent destruction hf.
+    case_eq (ident_eq id (dname d0)) ;
+    intro e ; rewrite e in h.
+    + inversion h as [ h' ]. subst. clear h.
+      destruct (ident_eq_spec id (dname d)).
+      * subst. destruct (ident_eq_spec (dname d) (dname d0)).
+        -- exfalso. easy.
+        -- easy.
+      * reflexivity.
+    + eapply IHΣ ; eassumption.
+Defined.
+
+Fixpoint weak_glob_type {Σ Γ t A} (h : Σ ;;; Γ |-w t : A) :
+  forall {d},
+    fresh_glob (dname d) Σ ->
+    (d::Σ) ;;; Γ |-w t : A
+
+with weak_glob_wf {Σ Γ} (h : wf Σ Γ) :
+  forall {d},
+    fresh_glob (dname d) Σ ->
+    wf (d::Σ) Γ.
+Proof.
+  (* weak_glob_type *)
+  - { dependent destruction h ; intros d fd.
+      all: try (econstructor ; try apply weak_glob_wf ;
+                try apply weak_glob_type ;
+                eassumption
+               ).
+      - eapply type_ProjT2 with (A3 := A1).
+        all: apply weak_glob_type ; eassumption.
+      - eapply type_Ax.
+        + eapply weak_glob_wf ; eassumption.
+        + cbn. erewrite ident_neq_fresh by eassumption.
+          assumption.
+    }
+
+  (* weak_glob_wf *)
+  - { dependent destruction h ; intros fd.
+      - constructor.
+      - econstructor.
+        + apply weak_glob_wf ; assumption.
+        + apply weak_glob_type ; eassumption.
+    }
+Defined.
+
+Corollary weak_glob_isType :
+  forall {Σ Γ A} (h : isType Σ Γ A) {d},
+    fresh_glob (dname d) Σ ->
+    isType (d::Σ) Γ A.
+Proof.
+  intros Σ Γ A h d hf.
+  destruct h as [s h].
+  exists s. eapply weak_glob_type ; eassumption.
+Defined.
+
+Fact type_ctx_closed_above :
+  forall {Σ Γ t T},
+    Σ ;;; Γ |-w t : T ->
+    closed_above #|Γ| t = true.
+Proof.
+  intros Σ Γ t T h.
+  dependent induction h.
+  all: try (cbn in * ; repeat erewrite_assumption ; reflexivity).
+  unfold closed_above. case_eq (n <? #|Γ|) ; intro e ; bprop e ; try myomega.
+  reflexivity.
+Defined.
+
+Fact typed_ax_type :
+  forall {Σ}, type_glob Σ ->
+  forall {id ty},
+    lookup_glob Σ id = Some ty ->
+    isType Σ [] ty.
+Proof.
+  intros Σ hg. dependent induction hg ; intros id ty h.
+  - cbn in h. discriminate h.
+  - cbn in h.
+    case_eq (ident_eq id (dname d)).
+    + intro e. rewrite e in h. inversion h. subst.
+      eapply weak_glob_isType ; eassumption.
+    + intro e. rewrite e in h.
+      specialize (IHhg _ _ h).
+      eapply weak_glob_isType ; eassumption.
+Defined.
+
+Fact type_ctxempty_closed :
+  forall {Σ t T},
+    Σ ;;; [] |-w t : T ->
+    closed t.
+Proof.
+  intros Σ t T h.
+  unfold closed. eapply @type_ctx_closed_above with (Γ := []). eassumption.
+Defined.
+
+Fact lift_ax_type :
+  forall {Σ},
+    type_glob Σ ->
+    forall {id ty},
+      lookup_glob Σ id = Some ty ->
+      forall n k, lift n k ty = ty.
+Proof.
+  intros Σ hg id ty isd n k.
+  destruct (typed_ax_type hg isd).
+  eapply closed_lift.
+  eapply type_ctxempty_closed. eassumption.
 Defined.
 
 Ltac ih h :=
@@ -108,185 +394,103 @@ with wf_lift {Σ Γ Δ Ξ} (h : wf Σ (Γ ,,, Ξ)) {struct h} :
   wf Σ (Γ ,,, Δ) ->
   wf Σ (Γ ,,, Δ ,,, lift_context #|Δ| Ξ)
 .
-(* Proof. *)
-(*   - { dependent destruction h ; intros hΣ hwf. *)
-(*       - cbn. case_eq (#|Ξ| <=? n) ; intro e ; bprop e. *)
-(*         + rewrite liftP3 by myomega. *)
-(*           replace (#|Δ| + S n)%nat with (S (#|Δ| + n)) by myomega. *)
-(*           eapply meta_conv. *)
-(*           * eapply type_Rel. *)
-(*             eapply wf_lift ; assumption. *)
-(*           * f_equal. f_equal. *)
-(*             erewrite 3!safe_nth_ge' *)
-(*               by (try rewrite lift_context_length ; myomega). *)
-(*             eapply safe_nth_cong_irr. *)
-(*             rewrite lift_context_length. myomega. *)
-(*         + eapply meta_conv. *)
-(*           * eapply type_Rel. eapply wf_lift ; assumption. *)
-(*           * erewrite 2!safe_nth_lt. *)
-(*             eapply lift_context_ex. *)
-(*       - cbn. apply type_Sort. now apply wf_lift. *)
-(*       - cbn. eapply type_Prod ; eih. *)
-(*       - cbn. eapply type_Lambda ; eih. *)
-(*       - cbn. *)
-(*         change (lift #|Δ| #|Ξ| (B {0 := u})) *)
-(*           with (lift #|Δ| (0 + #|Ξ|) (B { 0 := u })). *)
-(*         rewrite substP1. *)
-(*         eapply type_App ; eih. *)
-(*       - cbn. eapply type_Sum ; eih. *)
-(*       - cbn. eapply type_Pair ; eih. *)
-(*         change (#|Ξ|) with (0 + #|Ξ|)%nat. *)
-(*         rewrite substP1. reflexivity. *)
-(*       - cbn. eapply type_Pi1 ; eih. *)
-(*       - cbn. *)
-(*         change (#|Ξ|) with (0 + #|Ξ|)%nat. *)
-(*         rewrite substP1. cbn. *)
-(*         eapply type_Pi2 ; eih. *)
-(*       - cbn. apply type_Eq ; eih. *)
-(*       - cbn. eapply type_Refl ; eih. *)
-(*       - change (#|Ξ|) with (0 + #|Ξ|)%nat. *)
-(*         rewrite substP1. *)
-(*         replace (S (0 + #|Ξ|)) with (1 + #|Ξ|)%nat by myomega. *)
-(*         rewrite substP1. *)
-(*         cbn. eapply type_J ; try eih. *)
-(*         + cbn. unfold ssnoc. cbn. *)
-(*           f_equal. f_equal. *)
-(*           * replace (S #|Ξ|) with (1 + #|Ξ|)%nat by myomega. *)
-(*             apply liftP2. myomega. *)
-(*           * replace (S #|Ξ|) with (1 + #|Ξ|)%nat by myomega. *)
-(*             apply liftP2. myomega. *)
-(*         + replace (S (S #|Ξ|)) with (1 + (S (0 + #|Ξ|)))%nat by myomega. *)
-(*           rewrite <- substP1. *)
-(*           replace (1 + (0 + #|Ξ|))%nat with (S (0 + #|Ξ|))%nat by myomega. *)
-(*           change (sRefl (lift #|Δ| #|Ξ| A0) (lift #|Δ| #|Ξ| u)) *)
-(*             with (lift #|Δ| #|Ξ| (sRefl A0 u)). *)
-(*           rewrite <- substP1. reflexivity. *)
-(*       - cbn. eapply type_Transport ; eih. *)
-(*       - cbn. eapply type_Heq ; eih. *)
-(*       - cbn. eapply type_HeqToEq ; eih. *)
-(*       - cbn. eapply type_HeqRefl ; eih. *)
-(*       - cbn. eapply type_HeqSym ; eih. *)
-(*       - cbn. eapply @type_HeqTrans with (B := lift #|Δ| #|Ξ| B) (b := lift #|Δ| #|Ξ| b) ; eih. *)
-(*       - cbn. eapply type_HeqTransport ; eih. *)
-(*       - cbn. eapply type_CongProd ; try eih. *)
-(*         cbn. f_equal. *)
-(*         + rewrite <- liftP2 by myomega. *)
-(*           change (S #|Ξ|) with (0 + (S #|Ξ|))%nat at 1. *)
-(*           rewrite substP1. cbn. reflexivity. *)
-(*         + rewrite <- liftP2 by myomega. *)
-(*           change (S #|Ξ|) with (0 + (S #|Ξ|))%nat at 1. *)
-(*           rewrite substP1. cbn. reflexivity. *)
-(*       - cbn. eapply type_CongLambda ; try eih. *)
-(*         + cbn. f_equal. *)
-(*           * rewrite <- liftP2 by myomega. *)
-(*             change (S #|Ξ|) with (0 + (S #|Ξ|))%nat at 1. *)
-(*             rewrite substP1. cbn. reflexivity. *)
-(*           * rewrite <- liftP2 by myomega. *)
-(*             change (S #|Ξ|) with (0 + (S #|Ξ|))%nat at 1. *)
-(*             rewrite substP1. cbn. reflexivity. *)
-(*         + cbn. f_equal. *)
-(*           * rewrite <- liftP2 by myomega. *)
-(*             change (S #|Ξ|) with (0 + (S #|Ξ|))%nat at 1. *)
-(*             rewrite substP1. cbn. reflexivity. *)
-(*           * rewrite <- liftP2 by myomega. *)
-(*             change (S #|Ξ|) with (0 + (S #|Ξ|))%nat at 1. *)
-(*             rewrite substP1. cbn. reflexivity. *)
-(*           * rewrite <- liftP2 by myomega. *)
-(*             change (S #|Ξ|) with (0 + (S #|Ξ|))%nat at 1. *)
-(*             rewrite substP1. cbn. reflexivity. *)
-(*           * rewrite <- liftP2 by myomega. *)
-(*             change (S #|Ξ|) with (0 + (S #|Ξ|))%nat at 1. *)
-(*             rewrite substP1. cbn. reflexivity. *)
-(*       - cbn. *)
-(*         change (lift #|Δ| #|Ξ| (B1 {0 := v1})) *)
-(*           with (lift #|Δ| (0 + #|Ξ|) (B1 { 0 := v1 })). *)
-(*         change (lift #|Δ| #|Ξ| (B2 {0 := v2})) *)
-(*           with (lift #|Δ| (0 + #|Ξ|) (B2 { 0 := v2 })). *)
-(*         rewrite 2!substP1. *)
-(*         eapply type_CongApp ; eih. *)
-(*         cbn. f_equal. *)
-(*         + rewrite <- liftP2 by myomega. *)
-(*           change (S #|Ξ|) with (0 + (S #|Ξ|))%nat at 1. *)
-(*           rewrite substP1. cbn. reflexivity. *)
-(*         + rewrite <- liftP2 by myomega. *)
-(*           change (S #|Ξ|) with (0 + (S #|Ξ|))%nat at 1. *)
-(*           rewrite substP1. cbn. reflexivity. *)
-(*       - cbn. eapply type_CongSum ; try eih. *)
-(*         cbn. f_equal. *)
-(*         + rewrite <- liftP2 by myomega. *)
-(*           change (S #|Ξ|) with (0 + (S #|Ξ|))%nat at 1. *)
-(*           rewrite substP1. cbn. reflexivity. *)
-(*         + rewrite <- liftP2 by myomega. *)
-(*           change (S #|Ξ|) with (0 + (S #|Ξ|))%nat at 1. *)
-(*           rewrite substP1. cbn. reflexivity. *)
-(*       - cbn. eapply type_CongPair ; eih. *)
-(*         + cbn. f_equal. *)
-(*           * rewrite <- liftP2 by myomega. *)
-(*             change (S #|Ξ|) with (0 + (S #|Ξ|))%nat at 1. *)
-(*             rewrite substP1. cbn. reflexivity. *)
-(*           * rewrite <- liftP2 by myomega. *)
-(*             change (S #|Ξ|) with (0 + (S #|Ξ|))%nat at 1. *)
-(*             rewrite substP1. cbn. reflexivity. *)
-(*         + cbn. f_equal. *)
-(*           * change #|Ξ| with (0 + #|Ξ|)%nat. *)
-(*             rewrite substP1. reflexivity. *)
-(*           * change #|Ξ| with (0 + #|Ξ|)%nat. *)
-(*             rewrite substP1. reflexivity. *)
-(*         + change #|Ξ| with (0 + #|Ξ|)%nat. *)
-(*           rewrite substP1. reflexivity. *)
-(*         + change #|Ξ| with (0 + #|Ξ|)%nat. *)
-(*           rewrite substP1. reflexivity. *)
-(*       - cbn. eapply type_CongPi1 ; eih. *)
-(*         cbn. f_equal. *)
-(*         + rewrite <- liftP2 by myomega. *)
-(*           change (S #|Ξ|) with (0 + (S #|Ξ|))%nat at 1. *)
-(*           rewrite substP1. cbn. reflexivity. *)
-(*         + rewrite <- liftP2 by myomega. *)
-(*           change (S #|Ξ|) with (0 + (S #|Ξ|))%nat at 1. *)
-(*           rewrite substP1. cbn. reflexivity. *)
-(*       - cbn. *)
-(*         change #|Ξ| with (0 + #|Ξ|)%nat. *)
-(*         rewrite 2!substP1. *)
-(*         eapply type_CongPi2 ; eih. *)
-(*         cbn. f_equal. *)
-(*         + rewrite <- liftP2 by myomega. *)
-(*           change (S #|Ξ|) with (0 + (S #|Ξ|))%nat at 1. *)
-(*           rewrite substP1. cbn. reflexivity. *)
-(*         + rewrite <- liftP2 by myomega. *)
-(*           change (S #|Ξ|) with (0 + (S #|Ξ|))%nat at 1. *)
-(*           rewrite substP1. cbn. reflexivity. *)
-(*       - cbn. eapply type_CongEq ; eih. *)
-(*       - cbn. eapply type_CongRefl ; eih. *)
-(*       - cbn. eapply type_EqToHeq ; eih. *)
-(*       - cbn. eapply type_HeqTypeEq ; eih. *)
-(*       - cbn. eapply type_Pack ; eih. *)
-(*       - cbn. eapply @type_ProjT1 with (A2 := lift #|Δ| #|Ξ| A2) ; eih. *)
-(*       - cbn. eapply @type_ProjT2 with (A1 := lift #|Δ| #|Ξ| A1) ; eih. *)
-(*       - cbn. eapply type_ProjTe ; eih. *)
-(*       - cbn. erewrite lift_ax_type by eassumption. *)
-(*         eapply type_Ax. *)
-(*         + now apply wf_lift. *)
-(*         + assumption. *)
-(*       - eapply type_conv ; try eih. *)
-(*         eapply lift_conv. assumption. *)
-(*     } *)
+Proof.
+  - { dependent destruction h ; intros hΣ hwf.
+      - cbn. case_eq (#|Ξ| <=? n) ; intro e ; bprop e.
+        + rewrite liftP3 by myomega.
+          replace (#|Δ| + S n)%nat with (S (#|Δ| + n)) by myomega.
+          eapply meta_conv.
+          * eapply type_Rel.
+            eapply wf_lift ; assumption.
+          * f_equal. f_equal.
+            erewrite 3!safe_nth_ge'
+              by (try rewrite lift_context_length ; myomega).
+            eapply safe_nth_cong_irr.
+            rewrite lift_context_length. myomega.
+        + eapply meta_conv.
+          * eapply type_Rel. eapply wf_lift ; assumption.
+          * erewrite 2!safe_nth_lt.
+            eapply lift_context_ex.
+      - cbn. apply type_Sort. now apply wf_lift.
+      - cbn. eapply type_Prod ; eih.
+      - cbn. eapply type_Lambda ; eih.
+      - cbn.
+        change (lift #|Δ| #|Ξ| (B {0 := u}))
+          with (lift #|Δ| (0 + #|Ξ|) (B { 0 := u })).
+        rewrite substP1.
+        eapply type_App with (A := lift #|Δ| #|Ξ| A0) ; eih.
+      - cbn. eapply type_Sum ; eih.
+      - cbn. eapply type_Pair ; eih.
+        change (#|Ξ|) with (0 + #|Ξ|)%nat.
+        rewrite substP1. reflexivity.
+      - cbn. eapply type_Pi1 ; eih.
+      - cbn.
+        change (#|Ξ|) with (0 + #|Ξ|)%nat.
+        rewrite substP1. cbn.
+        eapply type_Pi2 ; eih.
+      - cbn. apply type_Eq ; eih.
+      - cbn. eapply type_Refl ; eih.
+      - change (#|Ξ|) with (0 + #|Ξ|)%nat.
+        rewrite substP1.
+        replace (S (0 + #|Ξ|)) with (1 + #|Ξ|)%nat by myomega.
+        rewrite substP1.
+        cbn. eapply type_J ; try eih.
+        + cbn. unfold snoc. cbn.
+          f_equal. f_equal.
+          * replace (S #|Ξ|) with (1 + #|Ξ|)%nat by myomega.
+            apply liftP2. myomega.
+          * replace (S #|Ξ|) with (1 + #|Ξ|)%nat by myomega.
+            apply liftP2. myomega.
+        + replace (S (S #|Ξ|)) with (1 + (S (0 + #|Ξ|)))%nat by myomega.
+          rewrite <- substP1.
+          replace (1 + (0 + #|Ξ|))%nat with (S (0 + #|Ξ|))%nat by myomega.
+          change (wRefl (lift #|Δ| #|Ξ| A0) (lift #|Δ| #|Ξ| u))
+            with (lift #|Δ| #|Ξ| (wRefl A0 u)).
+          rewrite <- substP1. reflexivity.
+      - cbn. eapply type_Transport ; eih.
+      - cbn.
+        change (lift #|Δ| #|Ξ| (B {0 := u}))
+          with (lift #|Δ| (0 + #|Ξ|) (B { 0 := u })).
+        change (lift #|Δ| #|Ξ| (t0 {0 := u}))
+          with (lift #|Δ| (0 + #|Ξ|) (t0 { 0 := u })).
+        rewrite 2!substP1.
+        eapply type_Beta ; eih.
+      - cbn. eapply type_K ; eih.
+      - cbn. eapply type_Funext ; eih.
+        cbn. f_equal. f_equal.
+        + f_equal. replace (S #|Ξ|) with (1 + #|Ξ|)%nat by myomega.
+            apply liftP2. myomega.
+        + f_equal. replace (S #|Ξ|) with (1 + #|Ξ|)%nat by myomega.
+            apply liftP2. myomega.
+      - cbn. eapply type_Heq ; eih.
+      - cbn. eapply type_HeqPair ; eih.
+      - cbn. eapply type_HeqTy ; eih.
+      - cbn. eapply type_HeqTm ; eih.
+      - cbn. eapply type_Pack ; eih.
+      - cbn. eapply @type_ProjT1 with (A2 := lift #|Δ| #|Ξ| A2) ; eih.
+      - cbn. eapply @type_ProjT2 with (A1 := lift #|Δ| #|Ξ| A1) ; eih.
+      - cbn. eapply type_ProjTe ; eih.
+      - cbn. erewrite lift_ax_type by eassumption.
+        eapply type_Ax.
+        + now apply wf_lift.
+        + assumption.
+    }
 
-(*   (* wf_lift *) *)
-(*   - { intros hg hwf. *)
-(*       destruct Ξ. *)
-(*       - cbn. assumption. *)
-(*       - dependent destruction h. *)
-(*         cbn. econstructor. *)
-(*         + apply wf_lift ; assumption. *)
-(*         + instantiate (1 := s0). cbn. change (sSort s0) with (lift #|Δ| #|Ξ| (sSort s0)). *)
-(*           apply type_lift ; assumption. *)
-(*     } *)
+  (* wf_lift *)
+  - { intros hg hwf.
+      destruct Ξ.
+      - cbn. assumption.
+      - dependent destruction h.
+        cbn. econstructor.
+        + apply wf_lift ; assumption.
+        + instantiate (1 := s). cbn. change (wSort s) with (lift #|Δ| #|Ξ| (wSort s)).
+          apply type_lift ; assumption.
+    }
 
-(*     Unshelve. *)
-(*     all: try rewrite !length_cat ; try rewrite length_cat in isdecl ; *)
-(*       try rewrite lift_context_length ; myomega. *)
-(* Defined. *)
-Admitted.
+    Unshelve.
+    all: try rewrite !length_cat ; try rewrite length_cat in isdecl ;
+      try rewrite lift_context_length ; myomega.
+Defined.
 
 Corollary typing_lift01 :
   forall {Σ Γ t A B s},
